### 课堂练习 ###
#### 练习1：证明如下等式：（1）$[\hat{A},\hat{B}\hat{C}]=[\hat{A},\hat{B}]\hat{C}+\hat{B}[\hat{A},\hat{C}]$；（2）$[\hat{A}\hat{B},\hat{C}]=\hat{A}[\hat{B},\hat{C}]+[\hat{A},\hat{C}]\hat{B}$
**证明**：因为：
$$
\begin{split} [\hat{A},\hat{B}\hat{C}] &= \hat{A}(\hat{B}\hat{C})-(\hat{B}\hat{C})\hat{A}=\hat{A}\hat{B}\hat{C}-\hat{B}\hat{C}\hat{A}+\hat{B}\hat{A}\hat{C}-\hat{B}\hat{A}\hat{C}=(\hat{A}\hat{B}\hat{C}-\hat{B}\hat{A}\hat{C})+(-\hat{B}\hat{C}\hat{A}+\hat{B}\hat{A}\hat{C}) \\ &= (\hat{A}\hat{B}-\hat{B}\hat{A})\hat{C}+\hat{B}(\hat{A}\hat{C}-\hat{C}\hat{A})=[\hat{A},\hat{B}]\hat{C}+\hat{B}[\hat{A},\hat{C}] \end{split}
$$
$$
\begin{split} [\hat{A}\hat{B},\hat{C}] &= (\hat{A}\hat{B})\hat{C}-\hat{C}(\hat{A}\hat{B})=\hat{A}\hat{B}\hat{C}-\hat{C}\hat{A}\hat{B}+\hat{A}\hat{C}\hat{B}-\hat{A}\hat{C}\hat{B}=(\hat{A}\hat{B}\hat{C}-\hat{A}\hat{C}\hat{B})+(-\hat{C}\hat{A}\hat{B}+\hat{A}\hat{C}\hat{B}) \\ &= \hat{A}(\hat{B}\hat{C}-\hat{C}\hat{B})+(\hat{A}\hat{C}-\hat{C}\hat{A})\hat{B}=\hat{A}[\hat{B},\hat{C}]+[\hat{A},\hat{C}]\hat{B} \end{split}
$$
故原题得证
#### 练习2：以$| s_x+ \rangle$和$| s_x- \rangle$为基矢来表示$| s_z \pm \rangle$和$| s_y \pm \rangle$ ####
**解**：我们知道$| s_x+ \rangle=\frac{1}{\sqrt{2}} (| s_z+ \rangle+| s_z- \rangle)$，$| s_x- \rangle=\frac{1}{\sqrt{2}} (| s_z+ \rangle-| s_z- \rangle)$，因此两式相加得$| s_x+ \rangle+| s_x- \rangle=\sqrt{2} | s_z+ \rangle$，即$| s_z+ \rangle=\frac{1}{\sqrt{2}} (| s_x+ \rangle+| s_x- \rangle)$；两式相减得$| s_x+ \rangle-| s_x- \rangle=\sqrt{2} | s_z- \rangle$，即$| s_z- \rangle=\frac{1}{\sqrt{2}} (| s_x+ \rangle-| s_x- \rangle)$。因此，$| s_z \pm \rangle$的表达式为$| s_z \pm \rangle=\frac{1}{\sqrt{2}} (| s_x+ \rangle \pm | s_x- \rangle)$。
我们再来看看$| s_y \pm \rangle$，由于$| s_y \pm \rangle=\frac{1}{\sqrt{2}}(| s_z+ \rangle \pm \mathrm{i} | s_z- \rangle)$，因此将上述的$| s_z \pm \rangle$的表达式代入，得
$$
| s_y+ \rangle=\frac{1}{\sqrt{2}}(| s_z+ \rangle+\mathrm{i}| s_z- \rangle)=\frac{1}{\sqrt{2}}[\frac{1}{\sqrt{2}}(| s_x+ \rangle+| s_x- \rangle)+\frac{\mathrm{i}}{\sqrt{2}}(| s_x+ \rangle-| s_x- \rangle)]=\frac{1+\mathrm{i}}{2} | s_x+ \rangle+\frac{1-\mathrm{i}}{2} | s_x- \rangle
$$
$$
| s_y- \rangle=\frac{1}{\sqrt{2}}(| s_z+ \rangle-\mathrm{i}| s_z- \rangle)=\frac{1}{\sqrt{2}}[\frac{1}{\sqrt{2}}(| s_x+ \rangle+| s_x- \rangle)-\frac{\mathrm{i}}{\sqrt{2}}(| s_x+ \rangle-| s_x- \rangle)]=\frac{1-\mathrm{i}}{2} | s_x+ \rangle+\frac{1+\mathrm{i}}{2} | s_x- \rangle
$$
从而$| s_y \pm \rangle=\frac{1 \pm \mathrm{i}}{2} | s_x+ \rangle+\frac{1 \mp \mathrm{i}}{2} | s_x- \rangle$